coq-proof/GammaHeapCorrespondence.v
@@ -13,8 +13,11 @@ Require Import HeapDefs.
 Reserved Notation "'gh:' g '|-' h 'OK'" (at level 40).
 Inductive Gamma_Heap_OK : Gamma -> Heap -> Prop :=
   | GH_Correspondence : forall (g : Gamma) (h : Heap),
-    ( forall (f : ID), Gamma_Contains g f = true /\
+    ( forall (f : ID), Gamma_Contains g f = true ->
       exists (Tf Tv : Unit) (z : nat),
-      Gamma_Get g f = Some Tf /\ FieldType h f = Tf /\ Tv <: Tf = true /\ FieldValue h f = Val Tv z ) ->
+        Gamma_Get g f = Some Tf /\
+        FieldType h f = Some Tf /\
+        Tv <: Tf = true /\
+        FieldValue h f = Some (Val Tv z) ) ->
     gh: g |- h OK
 where "'gh:' g '|-' h 'OK'" := (Gamma_Heap_OK g h).
